working on proofs of hashing & converting them to abstract maps.

src/NatMap.v
@@ -54,158 +54,85 @@ Module IntMapProperties := HintlessFMapFacts.WProperties_fun(Ordered_nat)(IntMap
 Definition singleton {T} (k : nat) (v : T) : IntMap.t T :=
   IntMap.add k v (IntMap.empty _).
 
-(*
-
-(** Other Lemmas **)
-(* these currently break the FMap abstraction, but they could be proved
- * using only the FMap abstraction
- *)
-
-
-Theorem elements_map : forall T U (F : T -> U) m,
-  IntMap.bst m ->
-  IntMap.elements (IntMap.map F m) = List.map (fun x => (fst x, F (snd x))) (IntMap.elements m).
-Proof.
-  clear. unfold IntMap.elements. do 4 intro. 
-  change (@nil (IntMap.key * U)) with (List.map (fun x => (fst x, F (snd x))) (@nil (IntMap.key * T))).
-  generalize (@nil (IntMap.key * T)).
-  induction m; simpl; intros; try reflexivity.
-  inversion H; subst; auto.
-  rewrite IHm2; eauto.
-  change (((k, F e) :: map (fun x : IntMap.key * T => (fst x, F (snd x))) (IntMap.elements_aux l m2)))
-    with (map (fun x : IntMap.key * T => (fst x, F (snd x))) ((k,e) :: (IntMap.elements_aux l m2))).
-  rewrite IHm1; eauto.
-Qed.
-
-Lemma elements_singleton : forall T k (v : T), 
-  IntMap.elements (singleton k v) = (k,v) :: nil.
-Proof.
-  unfold IntMap.empty. intros. reflexivity.
-Qed.
-
-
-Lemma find_elements_split : forall T k (v : T) m,
-  IntMap.find k m = Some v ->
-  exists ls, exists rs, IntMap.elements m = ls ++ (k,v) :: rs.
-Proof.
-  intros. apply IntMap.Proofs.find_2 in H.
-  eapply IntMap.Proofs.elements_mapsto in H.
-  eapply SetoidList.InA_split in H.
-  do 3 destruct H. destruct x0. intuition. 
-  destruct H0; simpl in *; subst. eauto.
-Qed.
-
-(*
-SearchAbout IntMap.elements.
-
-Lemma prove_elements : forall T (m : IntMap.t T) ls,
-  IntMap.bst m ->
-  (Sorted.Sorted (IntMap.Proofs.PX.ltk (elt:=T)) ls /\
-    (forall k v, IntMap.MapsTo k v m <-> SetoidList.InA  (IntMap.Proofs.PX.eqke (elt:=T))  (k, v) ls)) <->
-  IntMap.elements m = ls.
-Admitted.
-*)
-
-Lemma find_elements_remove : forall T k (v : T) m ls rs,
-  IntMap.bst m ->
-  IntMap.elements m = ls ++ (k,v) :: rs ->
-  IntMap.elements (IntMap.remove k m) = ls ++ rs.
-Proof.
-  intros. (*apply prove_elements in H0; auto. apply prove_elements.
-  intros. *)
-Admitted.
-
-Lemma elements_find : forall T k (v : T) m,
-  IntMap.find k m = Some v ->
-  exists x y, IntMap.elements m = x ++ (k,v) :: y.
-Proof.
-  clear. induction m; intros.
-  compute in H; congruence.
-  simpl in H. generalize (IntMap.Proofs.elements_node m1 m2 k0 e i nil).
-  repeat rewrite app_nil_r. intros. rewrite <- H0. clear H0.
-
-  destruct (Ordered_nat.compare k k0).
-  eapply IHm1 in H. do 2 destruct H. rewrite H.
-  exists x. exists (x0 ++ (k0,e) :: IntMap.elements m2). repeat rewrite app_ass; simpl. reflexivity.
-
-  inversion e0; inversion H; subst; do 2 eexists; reflexivity.
+(** Neither Properties nor Facts contains anything useful about 'map' **)
+Module MoreFMapFacts (FM : HintlessFMapInterface.S).
   
-  apply IHm2 in H. do 2 destruct H. rewrite H.
-  exists (IntMap.elements m1 ++ (k0,e) :: x). eexists. repeat rewrite app_ass; simpl. reflexivity.
-Qed.
+  Module PROPS := HintlessFMapFacts.WProperties_fun(FM.E) FM.
+  Module FACTS := HintlessFMapFacts.WFacts_fun FM.E FM.    
 
-Lemma elements_add_over : forall T k (v v' : T) m x y,
-  IntMap.elements m = x ++ (k,v) :: y ->
-  IntMap.elements (IntMap.add k v' m) = x ++ (k,v') :: y.
-Proof.
-  clear; induction m; intros.
-  destruct x; compute in H; congruence.          
-Admitted.
+  Definition union T :=
+    FM.fold (fun k (v : T) a => FM.add k v a).
 
-(* TODO: how do i instantiate the FMapFacts module?
-Require FSets.FMapFacts.
-Module IntMap_WS <:  FSets.FMapInterface.WS.
-  Module E := Ordered_nat.
-  Include IntMap.
-End IntMap_WS.
+  Lemma map_Empty : forall T U (F : T -> U) m,
+    FM.Empty m ->
+    FM.Empty (FM.map F m).
+  Proof.
+    intros.
+    unfold FM.Empty in *.
+    intros. intro.
+    eapply FACTS.map_mapsto_iff in H0. destruct H0; intuition. eauto.
+  Qed.
 
-Module Ordered_nat_Props := FSets.FMapFacts.OrdProperties IntMap.
-*)
-
-Lemma elements_add_new : forall T k (v : T) m,
-  IntMap.find k m = None ->
-  exists x y, IntMap.elements m = x ++ y /\ IntMap.elements (IntMap.add k v m) = x ++ (k,v) :: y.
-Proof.
-  intros.
-Admitted.
-
-
-(*
-Ltac reduce_nat_map :=
-  cbv beta iota zeta delta 
-    [ singleton
-      IntMap.height IntMap.cardinal IntMap.empty IntMap.is_empty
-      IntMap.mem IntMap.find IntMap.assert_false IntMap.create IntMap.bal
-      IntMap.add IntMap.remove_min IntMap.merge IntMap.remove IntMap.join
-      IntMap.t_left IntMap.t_opt IntMap.t_right
-
-      Int.Z_as_Int._0 Int.Z_as_Int._1 Int.Z_as_Int._2 Int.Z_as_Int._3
-      Int.Z_as_Int.plus Int.Z_as_Int.max
-      Int.Z_as_Int.gt_le_dec Int.Z_as_Int.ge_lt_dec
-
-      ZArith_dec.Z_gt_le_dec ZArith_dec.Z_ge_lt_dec ZArith_dec.Z_ge_dec
-      ZArith_dec.Z_gt_dec 
-      ZArith_dec.Zcompare_rec ZArith_dec.Zcompare_rect
-
-      BinInt.Z.add BinInt.Z.max BinInt.Z.pos_sub
-      BinInt.Z.double BinInt.Z.succ_double BinInt.Z.pred_double
+  Lemma union_empty : forall T m,
+    FM.Equal (union T m (FM.empty _)) m.
+  Proof.
+    intros. unfold union.
+    remember (FM.empty T).
+    apply PROPS.map_induction with (m := m); intros.
+      rewrite PROPS.fold_Empty; eauto with typeclass_instances. subst; auto.
+      unfold FM.Equal, FM.Empty in *. intros.
+      rewrite FACTS.empty_o. case_eq (FM.find y m0); intros; auto.
+      exfalso. eapply H. eapply FM.find_2; eauto.
       
-      BinInt.Z.compare
+    erewrite PROPS.fold_Add; eauto with typeclass_instances.
+    rewrite H. unfold PROPS.Add, FM.Equal in *. eauto.
+    
+    repeat (red; intros; subst).
+    repeat (rewrite FACTS.add_o).
+      destruct (FM.E.eq_dec k y); auto.
+      destruct (FM.E.eq_dec k' y); auto. rewrite <- e1 in e2. exfalso; auto.
+  Qed.
 
-      BinPos.Pos.add BinPos.Pos.compare 
-      BinPos.Pos.succ BinPos.Pos.compare_cont
+  Lemma map_fold' : forall T U (F : T -> U) (m : FM.t T) (m' : FM.t U),
+    FM.Equal (union _ (FM.map F m) m')
+             (FM.fold (fun k v a => FM.add k (F v) a) m m').              
+  Proof.
+    do 4 intro. unfold union.
+    eapply PROPS.map_induction with (m := m); intros.
+    symmetry.
+    rewrite PROPS.fold_Empty; eauto with typeclass_instances.
+    rewrite PROPS.fold_Empty; eauto with typeclass_instances. reflexivity.
+    eapply map_Empty; auto.
 
-      Compare_dec.nat_compare CompOpp 
+    symmetry; rewrite PROPS.fold_Add; eauto with typeclass_instances.
+      specialize (H m'0).
+      cut (PROPS.Add x (F e) (FM.map F m0) (FM.map F m')); intros.
+      symmetry. rewrite PROPS.fold_Add. 6: eapply H2. 2: eauto with typeclass_instances.
+      rewrite H. reflexivity.
+      
+      repeat (red; intros; subst). rewrite H3. rewrite H4. reflexivity.
+      repeat (red; intros; subst). repeat rewrite FACTS.add_o.
+      destruct (FM.E.eq_dec k y); destruct (FM.E.eq_dec k' y); eauto.
+      rewrite <- e1 in e2; exfalso; auto.
+      intro. apply FACTS.map_in_iff in H3. auto.
+      
+      unfold PROPS.Add in *; intros.
+      specialize (H1 y). repeat (rewrite FACTS.add_o || rewrite FACTS.map_o || rewrite H1).
+      unfold FACTS.option_map.
+      destruct (FM.E.eq_dec x y); auto.
 
-      Ordered_nat.compare
+      repeat (red; intros; subst). rewrite H3. rewrite H2. reflexivity.
+      repeat (red; intros; subst). repeat rewrite FACTS.add_o.
+      repeat match goal with 
+               | [ |- context [ FM.E.eq_dec ?X ?Y ] ] => destruct (FM.E.eq_dec X Y); auto
+             end.
+      rewrite <- e1 in e2; exfalso; auto.
+  Qed.
 
-      sumor_rec sumor_rect
-      sumbool_rec sumbool_rect
-      eq_ind_r 
-
-    ].
-
-
-Goal 
-  let m := singleton 10 10 in
-  let m := IntMap.add 1 1 m in
-  let m := IntMap.add 5 5 m in
-  let m := IntMap.add 3 3 m in
-  let m := IntMap.add 2 2 m in
-    let m := IntMap.remove 3 m in
-  Some 5 = IntMap.find 5 m /\
-  m = m.
-reduce_nat_map.
-Abort.
-*)
-*)
+  Lemma map_fold : forall T U (F : T -> U) m,
+    FM.Equal (FM.map F m)
+             (FM.fold (fun k v a => FM.add k (F v) a) m (FM.empty _)).
+  Proof.
+    intros. etransitivity. symmetry; apply union_empty. apply map_fold'. 
+  Qed.
+End MoreFMapFacts.
