src/Multimap.v
@@ -1,0 +1,137 @@
+Require Import HintlessFMapInterface HintlessFMapFacts.
+Require Import List.
+
+Set Implicit Arguments.
+Set Strict Implicit.
+
+Module Make (FM : S).
+  Module FM := FM.
+  Module FACTS := HintlessFMapFacts.WFacts_fun FM.E FM.
+  Module PROPS := HintlessFMapFacts.WProperties_fun FM.E FM.
+  
+  Lemma find_Empty : forall T (m : FM.t T) x,
+    FM.Empty m -> FM.find x m = None.
+  Proof.
+    intros.
+    apply PROPS.F.not_find_in_iff. 
+    unfold FM.In, FM.Empty in *. specialize (H x).
+    intro. destruct H0. eapply H. eauto.
+  Qed.
+
+  Section typed.
+    Variable T : Type.
+  
+    Definition mmap := FM.t (list T).
+
+    Definition empty : mmap := FM.empty _.
+
+    Definition mmap_add (k : FM.key) (v : T) (m : mmap) : mmap :=
+      match FM.find k m with
+        | None => FM.add k (v :: nil) m
+        | Some v' => FM.add k (v :: v') m
+      end.
+
+    Definition mmap_extend (k : FM.key) (v : list T) (m : mmap) : mmap :=
+      match FM.find k m with
+        | None => FM.add k v m
+        | Some v' => FM.add k (v ++ v') m
+      end.
+
+    Lemma Proper_mmap_extend : Proper (FM.E.eq ==> eq ==> FM.Equal ==> FM.Equal) mmap_extend.
+    Proof.
+      unfold mmap_extend.
+      repeat (red; intros; subst). rewrite H; rewrite H0. destruct (FM.find (elt:=list T) y y1); rewrite H; rewrite H0; auto.
+    Qed.
+      
+    Lemma transpose_neqkey_mmap_extend : PROPS.transpose_neqkey FM.Equal mmap_extend.
+    Proof.
+      unfold mmap_extend. repeat (red; intros; subst).
+      (repeat match goal with
+                | [ H : Some _ = Some _ |- _ ] => inversion H; clear H; subst
+                | [ H : _ = _ |- _ ] => rewrite H 
+                | [ H : _ = _ |- _ ] => rewrite H in *
+                | [ H : FM.E.eq _ _ |- _ ] => rewrite H 
+                | [ H : FM.E.eq _ _ |- _ ] => rewrite H in *
+                | [ H : context [ FM.find _ _ ] |- _ ] => 
+                  rewrite FACTS.add_o in H
+                | [ |- context [ FM.find ?k ?a ] ] =>
+                  match a with
+                    | match _ with 
+                        | Some _ => _
+                        | None => _
+                      end => fail 1
+                    | _ => case_eq (FM.find k a); intros
+                  end
+              end);
+      repeat match goal with
+               | [ H : ~ FM.E.eq ?X ?X |- _ ] => exfalso; apply H; reflexivity
+               | [ H : FM.E.eq _ _ |- _ ] => rewrite H 
+               | [ H : FM.E.eq _ _ |- _ ] => rewrite H in *
+               | [ H : Some _ = Some _ |- _ ] => inversion H ; clear H; subst
+               | [ H : context [ FM.E.eq_dec ?A ?B ] |- _ ] =>
+                 destruct (FM.E.eq_dec A B); try congruence
+             end.
+    Qed.
+    Existing Instance Proper_mmap_extend.
+    Existing Class PROPS.transpose_neqkey.
+    Existing Instance transpose_neqkey_mmap_extend.
+
+    Definition mmap_join : mmap -> mmap -> mmap :=
+      FM.fold mmap_extend.
+
+    Lemma mmap_join_o : forall (a b : mmap) x,
+      FM.find x (mmap_join a b) = 
+      match FM.find x a with
+        | Some a => 
+          match FM.find x b with
+            | Some b => Some (a ++ b)
+            | None => Some a
+          end
+        | None => FM.find x b 
+      end.
+    Proof.
+      clear. unfold mmap_join.
+      do 2 intro. apply PROPS.map_induction with (m := a); intros.
+      rewrite PROPS.fold_Empty; eauto with typeclass_instances.
+      symmetry.
+      repeat rewrite find_Empty by assumption; auto. 
+      
+      rewrite PROPS.fold_Add; try solve [ clear; eauto with typeclass_instances ]. 
+      unfold mmap_extend at 1. rewrite H.
+      apply PROPS.F.not_find_in_iff in H0. rewrite H0.
+
+      specialize (H1 x0). rewrite H1.
+      case_eq (FM.find x b); intros; rewrite FACTS.add_o; destruct (FM.E.eq_dec x x0); 
+        try rewrite H;
+          repeat match goal with
+                   | [ H : FM.E.eq _ _ |- _ ] => rewrite H in *; clear H
+                   | [ H : ~FM.E.eq ?X ?X |- _ ] => exfalso; apply H; reflexivity
+                   | [ H : _ = _ |- _ ] => rewrite H
+                   | [ |- context [ FM.E.eq_dec ?X ?Y ] ] =>
+                     destruct (FM.E.eq_dec X Y); try congruence
+                   | _ => rewrite FACTS.add_o in *
+                 end.
+    Qed.
+
+    Lemma mmap_join_remove_acc : forall k (a b : mmap),
+      ~FM.In k a ->
+      FM.Equal (FM.remove k (mmap_join a b)) (mmap_join a (FM.remove k b)).
+    Proof.
+      unfold FM.Equal. intros.
+      repeat (rewrite FACTS.remove_o || rewrite mmap_join_o).
+      destruct (FM.E.eq_dec k y); try reflexivity.
+      apply PROPS.F.not_find_in_iff in H.
+      rewrite e in *.
+      rewrite H. reflexivity. 
+    Qed.
+     
+  End typed.
+
+  Definition mmap_map T U (F : T -> U) : mmap T -> mmap U :=
+    FM.map (map F).
+
+  Definition mmap_mapi T U (F : FM.key -> T -> U) : mmap T -> mmap U :=
+    FM.mapi (fun k => map (F k)).
+
+
+End Make.
